More proofs about history produce

nondeterministic_dataflow/Operator.thy
@@ -1,4 +1,4 @@
-section \<open>Operators, trace model, history model, cleaned predicate, and welltyped predicate\<close>
+text \<open>Operators, trace model, history model, cleaned predicate, and welltyped predicate\<close>
 
 theory Operator
 
@@ -17,14 +17,14 @@ code_lazy_type llist
 
 datatype (discs_sels) 'd observation = Observed (obs: 'd) | EOB | EOS
 codatatype (inputs: 'ip, outputs: 'op, dead 'd) op =
-    Read 'ip "'d observation \<Rightarrow> ('ip, 'op, 'd) op"
+  Read 'ip "'d observation \<Rightarrow> ('ip, 'op, 'd) op"
   | Write "('ip, 'op, 'd) op" 'op 'd
   | End
 
 type_synonym 'd channel = "'d llist"
 
 code_lazy_type op
- 
+
 fun chd where
   "chd LNil = EOS"
 | "chd (LCons x lxs) = Observed x"
@@ -33,336 +33,6 @@ abbreviation ctl :: "'d channel \<Rightarrow> 'd channel" where "ctl \<equiv> lt
 
 abbreviation CHD :: "'a \<Rightarrow> ('a \<Rightarrow> 'd channel) \<Rightarrow> 'd observation" where "CHD p lxs \<equiv> chd (lxs p)"
 abbreviation CTL :: "'a \<Rightarrow> ('a \<Rightarrow> 'd channel) \<Rightarrow> ('a \<Rightarrow> 'd channel)" where "CTL p lxs \<equiv> lxs(p := ctl (lxs p))"
-
-section\<open>Trace model basics\<close>
-datatype ('a, 'b) IO = Inp (proji: 'a) | Out (projo: 'b)
-
-coinductive traced where
-  Read: "traced (fuel(p := n)) (f (Observed x)) lxs \<Longrightarrow> traced fuel (Read p f) (LCons (Inp p, Observed x) lxs)"
-| ReadEOS: "traced (fuel(p := n)) (f EOS) lxs \<Longrightarrow> traced fuel (Read p f) (LCons (Inp p, EOS) lxs)"
-| ReadEOB: "fuel p = Suc n \<Longrightarrow> traced (fuel(p := n)) (f EOB) lxs \<Longrightarrow> traced fuel (Read p f) (LCons (Inp p, EOB) lxs)"
-| Write: "traced fuel op lxs \<Longrightarrow> traced fuel (Write op p x) (LCons (Out p, Observed x) lxs)"
-| End: "traced fuel End LNil"
-
-inductive_cases traced_EndE[elim!]: "traced m End lxs"
-inductive_cases traced_WriteE[elim!]: "traced m (Write op p' x) lxs"
-inductive_cases traced_ReadE[elim!]: "traced m (Read p' f) lxs"
-
-definition "traces m op = {lxs. traced m op lxs}"
-
-lemma traces_Read[simp]:
-  "traces m (Read p f) = (\<Union>x. LCons (Inp p, Observed x) ` (\<Union>n. traces (m(p := n)) (f (Observed x)))) \<union>
-                       LCons (Inp p, EOB) ` (case m p of Suc n \<Rightarrow> traces (m(p := n)) (f EOB) | _ \<Rightarrow> {}) \<union>
-                       LCons (Inp p, EOS) ` (\<Union>n. traces (m(p := n)) (f EOS))"
-  by (auto simp: traces_def image_iff intro: traced.intros split: nat.splits)
-
-lemma traces_Write[simp]:
-  "traces m (Write op p x) = LCons (Out p, Observed x) ` traces m op"
-  by (auto simp: traces_def intro: traced.intros)
-
-lemma traces_End[simp]:
-  "traces m End = {LNil}"
-  by (auto simp: traces_def intro: traced.intros)
-
-corec traced_wit where
-  "traced_wit op = (case op of
-    Read p f \<Rightarrow> LCons (Inp p, EOS) (traced_wit (f EOS))
-  | Write op' p' x \<Rightarrow> LCons (Out p', Observed x) (traced_wit op')
-  | End \<Rightarrow> LNil)"
-
-lemma lset_traced_wit: "t \<in> lset (traced_wit op) \<Longrightarrow> (\<exists>p \<in> inputs op. t = (Inp p, EOS)) \<or> (\<exists>q \<in> outputs op. \<exists>x. t = (Out q, Observed x))"
-  apply (induction t "traced_wit op" arbitrary: op rule: llist.set_induct)
-  apply (subst (asm) traced_wit.code)
-  apply (auto split: op.splits) []
-  apply (subst (asm) (2) traced_wit.code)
-  apply (fastforce split: op.splits) []
-  done
-
-definition agree :: "('l \<Rightarrow> 'l' \<Rightarrow> bool) \<Rightarrow> ('l \<times> 'c) llist \<Rightarrow> ('l' \<times> 'c) llist \<Rightarrow> bool" where
-  "agree R lxs lys = llist_all2 (rel_prod R (=)) (lfilter (Domainp R o fst) lxs) (lfilter (Rangep R o fst) lys)"
-
-
-definition "lproject R ios = (\<lambda>p. lmap (obs o snd) (lfilter (\<lambda>qx. case qx of (q, Observed x) \<Rightarrow> R p q | _ \<Rightarrow> False) ios))"
-
-lemma lproject_LNil[simp]: "lproject R LNil = (\<lambda>p. LNil)"
-  by (simp add: lproject_def)
-
-lemma lproject_LCons[simp]: "lproject R (LCons (q, Observed x) lxs) =
-  (\<lambda>p. if R p q then LCons x (lproject R lxs p) else lproject R lxs p)"
-  "lproject R (LCons (q, EOS) lxs) = lproject R lxs"
-  "lproject R (LCons (q, EOB) lxs) = lproject R lxs"
-  by (auto simp add: lproject_def)
-
-lemma lproject_empty_conv:
-  "lproject R lxs p = LNil \<longleftrightarrow> (\<forall>q x. (q, Observed x) \<in> lset lxs \<longrightarrow> \<not> R p q)"
-  "LNil = lproject R lxs p \<longleftrightarrow> (\<forall>q x. (q, Observed x) \<in> lset lxs \<longrightarrow> \<not> R p q)"
-  by (force simp: lproject_def lmap_eq_LNil LNil_eq_lmap lfilter_empty_conv
-    split: observation.splits)+
-
-lemma lproject_False: 
-  "(\<And>q x. (q, Observed x) \<in> lset lxs \<Longrightarrow> \<not> R p q) \<Longrightarrow> lproject R lxs p = LNil"
-  by (simp add: lproject_empty_conv)
-
-lemma lproject_False_weak: 
-  "(\<And>qx. qx \<in> lset lxs \<Longrightarrow> \<not> R p (fst qx)) \<Longrightarrow> lproject R lxs p = LNil"
-  by (force simp add: lproject_empty_conv)
-
-section\<open>Cleaned operators\<close>
-
-coinductive cleaned where
-  cleaned_Read[intro]: "p \<notin> inputs (f EOS) \<Longrightarrow> (\<And>x. cleaned (f x)) \<Longrightarrow>  cleaned (Read p f)"
-| cleaned_Write[intro]: "cleaned op \<Longrightarrow> cleaned (Write op q x)"
-| cleaned_End[iff]: "cleaned End"
-
-inductive_cases cleaned_ReadE[elim!]: "cleaned (Read p f)"
-inductive_cases cleaned_WriteE[elim!]: "cleaned (Write op q x)"
-inductive_cases cleaned_EndE[elim!]: "cleaned End"
-
-inductive cleaned_cong for R where
-  cc_base: "R op \<Longrightarrow> cleaned_cong R op"
-| cc_cleaned: "cleaned op \<Longrightarrow> cleaned_cong R op"
-| cc_read: "p \<notin> inputs (f EOS) \<Longrightarrow> (\<And>x. cleaned_cong R (f x)) \<Longrightarrow> cleaned_cong R (Read p f)"
-| cc_write: "cleaned_cong R op \<Longrightarrow> cleaned_cong R (Write op q x)"
-
-lemma cleaned_coinduct_upto: "X op \<Longrightarrow>
-  (\<And>op. X op \<Longrightarrow> (\<exists>p f. op = Read p f \<and> p \<notin> inputs (f EOS) \<and> (\<forall>x. cleaned_cong X (f x))) \<or> (\<exists>op' q x. op = Write op' q x \<and> (cleaned_cong X op')) \<or> op = End) \<Longrightarrow>
-  cleaned op"
-  apply (rule cleaned.coinduct[where X="cleaned_cong X"])
-   apply (erule cleaned_cong.intros)
-  apply (erule thin_rl)
-  subgoal premises prems for op
-    using prems(2)
-    apply (induct op rule: cleaned_cong.induct)
-    subgoal for op
-      by (auto dest: prems(1))
-    subgoal for op
-      by (cases op) auto
-    subgoal for f p
-      by auto
-    subgoal for f p
-      by auto
-    done
-  done
-
-lemma ldropn_LConsD: "ldropn n xs = LCons x ys \<Longrightarrow> x \<in> lset xs"
-  by (metis in_lset_ldropnD lset_intros(1))
-
-lemma non_input_traces: "t \<in> lset lxs \<Longrightarrow> t = (Inp p, y) \<Longrightarrow> p \<notin> inputs op \<Longrightarrow> lxs \<in> traces m op \<Longrightarrow> False"
-  apply (induct t lxs arbitrary: m op rule: llist.set_induct)
-  subgoal for t lxs m op
-    apply (cases op; auto)
-    done
-  subgoal for t lxs x m op
-    apply (cases op; auto split: nat.splits)
-    done
-  done
-
-lemma cleaned_traced_gen:
-  "cleaned op \<Longrightarrow> traced m op (rev ps @@- lxs) \<Longrightarrow> alw (wow ((=) (Inp p, EOS)) imp nxt (alw (wow (\<lambda>t. fst t \<noteq> Inp p)))) ps lxs"
-  apply (coinduction arbitrary: m op ps lxs)
-  subgoal for m op ps lxs
-    apply (cases lxs)
-     apply simp_all
-    subgoal for x lxs'
-      apply (intro conjI impI disjI1; blast?)
-      apply (induct ps arbitrary: op m rule: rev_induct)
-       apply simp
-      apply (erule traced.cases; simp)
-       apply (erule cleaned.cases; simp)
-       apply (auto simp: alw_iff_ldropn wow_alt dest!: ldropn_LConsD dest: non_input_traces[unfolded traces_def] split: llist.splits) []
-      apply simp
-      apply (erule traced.cases; simp)
-         apply (erule cleaned.cases; auto simp add: alw_iff_ldropn wow_alt)+
-      done
-    done
-  done
-
-lemma cleaned_traced:
-  "cleaned op \<Longrightarrow> traced m op lxs \<Longrightarrow> alw (wow ((=) (Inp p, EOS)) imp nxt (alw (wow (\<lambda>t. fst t \<noteq> Inp p)))) [] lxs"
-  using cleaned_traced_gen[where ps = "[]"] by simp
-
-section\<open>Full abstraction\<close>
-
-lemma traced_traced_wit: "traced m op (traced_wit op)"
-  apply (coinduction arbitrary: op m)
-  apply (subst (1 3 5 7) traced_wit.code)
-  apply (auto split: op.splits dest: lset_traced_wit simp: traced_wit.code[where op=End])
-  done
-
-lemma traces_nonempty: "traces m op \<noteq> {}"
-  by (auto simp: traces_def intro!: traced_traced_wit)
-
-lemma traces_op_eqI: "(\<Union>m. traces m op) = (\<Union>m. traces m op') \<Longrightarrow> op = op'"
-  apply (coinduction arbitrary: op op')
-  subgoal for op op'
-    apply (cases op; cases op')
-            apply (simp_all add: rel_fun_def set_eq_iff split: nat.splits)
-    subgoal for p f p' f'
-      apply (rule context_conjI)
-      subgoal
-        apply (drule spec[of _ "LCons (Inp p, EOS) (traced_wit (f EOS))"])
-        apply simp
-        apply (drule iffD1)
-         apply (rule exI[of _ "\<lambda>_. 0"])
-         apply simp
-        apply (rule disjI2)
-         apply (rule imageI)
-         apply (auto dest: lset_traced_wit simp: traces_def traced_traced_wit) []
-        apply (erule exE disjE conjE)+
-         apply (simp_all add: gr0_conv_Suc image_iff)
-        done
-      subgoal
-        apply safe
-        subgoal for x lxs m
-          apply (drule spec[of _ "LCons (Inp p, x) lxs"])
-          apply (drule iffD1)
-          apply (rule exI[of _ "m(p := Suc (m p))"])
-           apply (cases x; auto simp: image_iff dest: non_input_traces intro: exI[of _ "m p"]) []
-          apply (erule exE conjE disjE)+
-           apply (auto simp add: gr0_conv_Suc image_iff)
-          done
-        subgoal for x lxs m
-          apply (drule spec[of _ "LCons (Inp p', x) lxs"])
-          apply (drule iffD2)
-          apply (rule exI[of _ "m(p' := Suc (m p'))"])
-           apply (cases x; auto simp: image_iff dest: non_input_traces intro: exI[of _ "m p'"]) []
-          apply (erule exE conjE disjE)+
-           apply (auto simp add: gr0_conv_Suc image_iff)
-          done
-        done
-      done
-    subgoal
-      apply (auto simp: set_eq_iff image_iff)
-      apply (metis (no_types, lifting) IO.distinct(1) llist.inject mem_Collect_eq prod.inject traced_traced_wit traces_def)
-      done
-    subgoal
-      apply (auto dest!: spec[of _ LNil] simp: gr0_conv_Suc)
-      done
-    subgoal
-      apply (auto simp: set_eq_iff image_iff)
-      apply (metis (no_types, lifting) IO.distinct(1) llist.inject mem_Collect_eq prod.inject traced_traced_wit traces_def)
-      done
-    subgoal for op1 p1 x1 op2 p2 x2
-      apply auto
-      subgoal for lxs m
-        apply (drule spec[of _ "LCons (Out p1, Observed x1) lxs"])
-        apply auto
-        done
-      subgoal for lxs m
-        apply (drule spec[of _ "LCons (Out p2, Observed x2) lxs"])
-        apply auto
-        done
-      subgoal
-        apply (drule spec[of _ "LCons (Out p1, Observed x1) (traced_wit op1)"])
-        apply (auto simp: traced_traced_wit traces_def)
-        done
-      subgoal
-        apply (drule spec[of _ "LCons (Out p1, Observed x1) (traced_wit op1)"])
-        apply (auto simp: traced_traced_wit traces_def)
-        done
-      done
-    subgoal
-      apply (auto simp: set_eq_iff image_iff)
-      done
-    subgoal
-      apply (auto dest!: spec[of _ LNil] simp: gr0_conv_Suc)
-      done
-    subgoal
-      apply (auto simp: set_eq_iff image_iff)
-      done
-    done
-  done
-
-section\<open>Produce function\<close>
-
-inductive producing for p where
-  "producing p End lxs 0"
-| "producing p (Write _ p _) lxs 0"
-| "producing p (f (CHD p' lxs)) (CTL p' lxs) i \<Longrightarrow> producing p (Read p' f) lxs (Suc i)"
-| "p \<noteq> p' \<Longrightarrow> producing p op lxs i \<Longrightarrow> producing p (Write op p' x) lxs (Suc i)"
-
-inductive_cases producing_EndE[elim!]: "producing p End lxs n"
-inductive_cases producing_WriteE[elim!]: "producing p (Write op p' x) lxs n"
-inductive_cases producing_ReadE[elim!]: "producing p (Read p' f) lxs n"
-
-lemma producing_inject: "producing p op lxs i \<Longrightarrow> producing p op lxs j \<Longrightarrow> i = j"
-  by (induct op lxs i arbitrary: j rule: producing.induct) fastforce+
-
-lemma The_producing: "producing p op lxs i \<Longrightarrow> The (producing p op lxs) = i"
-  using producing_inject by fast
-
-corecursive produce where
-  "produce op lxs p = (let produce' = (\<lambda>op' lxs'. if \<exists>i. producing p op lxs i then produce op' lxs' p else LNil) in case op of
-    Read p' f \<Rightarrow> (produce' (f (CHD p' lxs)) (CTL p' lxs))
-  | Write op' p' x \<Rightarrow> (if p = p' then LCons x (produce op' lxs p) else produce' op' lxs)
-  | End \<Rightarrow> LNil)"
-  by (relation "measure (\<lambda>(op, lxs, p). THE i. producing p op lxs i)")
-    (auto 0 3 simp: The_producing del: producing_ReadE producing_WriteE elim: producing.cases)
-
-lemma produce_code[code]:
-  "produce op lxs p = (case op of
-    Read p' f \<Rightarrow> produce (f (CHD p' lxs)) (CTL p' lxs) p
-  | Write op' p' x \<Rightarrow> (if p = p' then LCons x (produce op' lxs p) else produce op' lxs p)
-  | End \<Rightarrow> LNil)"
-  apply (subst produce.code)
-  apply (simp split: op.splits if_splits)
-  apply safe
-  subgoal for p' f
-    by (subst produce.code) (auto 0 5 split: op.splits intro: producing.intros)
-  subgoal for op p x
-    by (subst produce.code) (auto 0 4 split: op.splits intro: producing.intros)
-  done
-
-simps_of_case produce_simps[simp]: produce_code
-
-(* lemma produced_produce: "produced m op lxs (produce op lxs)"
-  apply (coinduction arbitrary: m op lxs)
-  subgoal for m op lxs
-    by (cases op) (force simp: muted_def muted_produce[unfolded muted_def])+
-  done *)
-
-section\<open>Buffer infrastrcuture\<close>
-
-datatype 'd buf = BEmpty | BEnded | BCons 'd "'d buf"
-
-fun bhd where
-  "bhd BEmpty = EOB"
-| "bhd BEnded = EOS"
-| "bhd (BCons x xs) = Observed x"
-
-fun btl where
-  "btl BEmpty = BEmpty"
-| "btl BEnded = BEnded"
-| "btl (BCons x xs) = xs"
-
-fun bend where
-  "bend BEmpty = BEnded"
-| "bend BEnded = BEnded"
-| "bend (BCons xs xss) = BCons xs (bend xss)"
-
-fun benq where
-  "benq x BEmpty = BCons x BEmpty"
-| "benq x BEnded = BCons x BEnded"
-| "benq x (BCons y ys) = BCons y (benq x ys)"
-
-abbreviation BHD :: "'a \<Rightarrow> ('a \<Rightarrow> 'd buf) \<Rightarrow> 'd observation" where "BHD p buf \<equiv> bhd (buf p)"
-abbreviation (input) BUPD where "BUPD f p buf \<equiv> buf(p := f (buf p))"
-abbreviation BTL :: "'a \<Rightarrow> ('a \<Rightarrow> 'd buf) \<Rightarrow> ('a \<Rightarrow> 'd buf)" where "BTL \<equiv> BUPD btl"
-abbreviation BENQ :: "'a \<Rightarrow> 'd \<Rightarrow> ('a \<Rightarrow> 'd buf) \<Rightarrow> ('a \<Rightarrow> 'd buf)" where "BENQ p x buf \<equiv> BUPD (benq x) p buf"
-abbreviation BENQ_TL :: "'a \<Rightarrow> 'd \<Rightarrow> ('a \<Rightarrow> 'd buf) \<Rightarrow> ('a \<Rightarrow> 'd buf)" where "BENQ_TL p x buf \<equiv> BUPD (btl o benq x) p buf"
-
-fun bapp where
-  "bapp BEmpty lxs = lxs"
-| "bapp BEnded lxs = LNil"
-| "bapp (BCons x xs) lxs = LCons x (bapp xs lxs)"
-
-definition "extend A buf R lxs lys =
-  (\<exists>lzs. R lxs (case_sum (lys o Inl) lzs) \<and> (\<forall>p. lys (Inr p) = (if p \<in> A then bapp (buf p) (lzs p) else lzs p)))"
-
-lemma extend_empty: "extend {} buf R = R"
-  using arg_cong2[of x x "case_sum (f o Inl) (f o Inr)" f R for x f, unfolded o_def, OF refl surjective_sum]
-  by (auto simp: extend_def o_def fun_eq_iff[of "extend _ _ _"] fun_eq_iff[of "extend _ _ _ _"]
-    simp flip: fun_eq_iff split: sum.splits)
 
 section\<open>Inputs measure\<close>
 
@@ -385,8 +55,8 @@ definition "input_depth p op = (LEAST n. input_at p op n)"
 lemma input_depth_Read: "p \<in> inputs op \<Longrightarrow> input_depth p op = 0 \<longleftrightarrow> (\<exists>f. op = Read p f)"
   unfolding input_depth_def
   apply (cases op)
-  apply (auto intro: input_at.intros Least_eq_0)
-  apply (metis LeastI_ex Zero_not_Suc input_at.simps inputs_input_at op.inject(1))
+    apply (auto intro: input_at.intros Least_eq_0)
+   apply (metis LeastI_ex Zero_not_Suc input_at.simps inputs_input_at op.inject(1))
   apply (metis input_at.simps inputs_input_at op.simps(4) wellorder_Least_lemma(1) zero_less_Suc)
   done
 
@@ -520,17 +190,477 @@ lemma output_depth_Write_simp_diff[simp]:
   "\<exists>x. p \<in> outputs op \<Longrightarrow>
    p \<noteq> p' \<Longrightarrow>
    output_depth p (Write op p' x) = Suc (output_depth p op)"
- unfolding output_depth_def outputs_alt
+  unfolding output_depth_def outputs_alt
   apply (elim exE)
   subgoal for x n
     apply (rule Least_Suc2[where n="Suc n"])
-    defer
+       defer
        apply assumption
     using output_at.cases apply force
-    apply (smt (verit, ccfv_threshold) diff_Suc_1 op.distinct(1) op.inject(2) output_at.cases output_at.intros(2))
+     apply (smt (verit, ccfv_threshold) diff_Suc_1 op.distinct(1) op.inject(2) output_at.cases output_at.intros(2))
     apply (auto intro: output_at.intros)
     done
   done
+
+
+section\<open>Trace model basics\<close>
+datatype ('a, 'b) IO = Inp (proji: 'a) | Out (projo: 'b)
+
+coinductive traced where
+  Read: "traced (fuel(p := n)) (f (Observed x)) lxs \<Longrightarrow> traced fuel (Read p f) (LCons (Inp p, Observed x) lxs)"
+| ReadEOS: "traced (fuel(p := n)) (f EOS) lxs \<Longrightarrow> traced fuel (Read p f) (LCons (Inp p, EOS) lxs)"
+| ReadEOB: "fuel p = Suc n \<Longrightarrow> traced (fuel(p := n)) (f EOB) lxs \<Longrightarrow> traced fuel (Read p f) (LCons (Inp p, EOB) lxs)"
+| Write: "traced fuel op lxs \<Longrightarrow> traced fuel (Write op p x) (LCons (Out p, Observed x) lxs)"
+| End: "traced fuel End LNil"
+
+inductive_cases traced_EndE[elim!]: "traced m End lxs"
+inductive_cases traced_WriteE[elim!]: "traced m (Write op p' x) lxs"
+inductive_cases traced_ReadE[elim!]: "traced m (Read p' f) lxs"
+
+definition "traces m op = {lxs. traced m op lxs}"
+
+lemma traces_Read[simp]:
+  "traces m (Read p f) = (\<Union>x. LCons (Inp p, Observed x) ` (\<Union>n. traces (m(p := n)) (f (Observed x)))) \<union>
+                       LCons (Inp p, EOB) ` (case m p of Suc n \<Rightarrow> traces (m(p := n)) (f EOB) | _ \<Rightarrow> {}) \<union>
+                       LCons (Inp p, EOS) ` (\<Union>n. traces (m(p := n)) (f EOS))"
+  by (auto simp: traces_def image_iff intro: traced.intros split: nat.splits)
+
+lemma traces_Write[simp]:
+  "traces m (Write op p x) = LCons (Out p, Observed x) ` traces m op"
+  by (auto simp: traces_def intro: traced.intros)
+
+lemma traces_End[simp]:
+  "traces m End = {LNil}"
+  by (auto simp: traces_def intro: traced.intros)
+
+corec traced_wit where
+  "traced_wit op = (case op of
+    Read p f \<Rightarrow> LCons (Inp p, EOS) (traced_wit (f EOS))
+  | Write op' p' x \<Rightarrow> LCons (Out p', Observed x) (traced_wit op')
+  | End \<Rightarrow> LNil)"
+
+lemma lset_traced_wit: "t \<in> lset (traced_wit op) \<Longrightarrow> (\<exists>p \<in> inputs op. t = (Inp p, EOS)) \<or> (\<exists>q \<in> outputs op. \<exists>x. t = (Out q, Observed x))"
+  apply (induction t "traced_wit op" arbitrary: op rule: llist.set_induct)
+   apply (subst (asm) traced_wit.code)
+   apply (auto split: op.splits) []
+  apply (subst (asm) (2) traced_wit.code)
+  apply (fastforce split: op.splits) []
+  done
+
+definition agree :: "('l \<Rightarrow> 'l' \<Rightarrow> bool) \<Rightarrow> ('l \<times> 'c) llist \<Rightarrow> ('l' \<times> 'c) llist \<Rightarrow> bool" where
+  "agree R lxs lys = llist_all2 (rel_prod R (=)) (lfilter (Domainp R o fst) lxs) (lfilter (Rangep R o fst) lys)"
+
+
+definition "lproject R ios = (\<lambda>p. lmap (obs o snd) (lfilter (\<lambda>qx. case qx of (q, Observed x) \<Rightarrow> R p q | _ \<Rightarrow> False) ios))"
+
+lemma lproject_LNil[simp]: "lproject R LNil = (\<lambda>p. LNil)"
+  by (simp add: lproject_def)
+
+lemma lproject_LCons[simp]: "lproject R (LCons (q, Observed x) lxs) =
+  (\<lambda>p. if R p q then LCons x (lproject R lxs p) else lproject R lxs p)"
+  "lproject R (LCons (q, EOS) lxs) = lproject R lxs"
+  "lproject R (LCons (q, EOB) lxs) = lproject R lxs"
+  by (auto simp add: lproject_def)
+
+lemma lproject_LCons_False[simp]:
+  "\<not> P p p' \<Longrightarrow>
+   lproject P (LCons (p', x) lxs) p = lproject P lxs p"
+  apply (cases x)
+    apply auto
+  done
+
+lemma lproject_empty_conv:
+  "lproject R lxs p = LNil \<longleftrightarrow> (\<forall>q x. (q, Observed x) \<in> lset lxs \<longrightarrow> \<not> R p q)"
+  "LNil = lproject R lxs p \<longleftrightarrow> (\<forall>q x. (q, Observed x) \<in> lset lxs \<longrightarrow> \<not> R p q)"
+  by (force simp: lproject_def lmap_eq_LNil LNil_eq_lmap lfilter_empty_conv
+      split: observation.splits)+
+
+lemma lproject_False: 
+  "(\<And>q x. (q, Observed x) \<in> lset lxs \<Longrightarrow> \<not> R p q) \<Longrightarrow> lproject R lxs p = LNil"
+  by (simp add: lproject_empty_conv)
+
+lemma lproject_False_weak: 
+  "(\<And>qx. qx \<in> lset lxs \<Longrightarrow> \<not> R p (fst qx)) \<Longrightarrow> lproject R lxs p = LNil"
+  by (force simp add: lproject_empty_conv)
+
+section\<open>Cleaned predicate\<close>
+
+coinductive cleaned where
+  cleaned_Read[intro]: "p \<notin> inputs (f EOS) \<Longrightarrow> (\<And>x. cleaned (f x)) \<Longrightarrow>  cleaned (Read p f)"
+| cleaned_Write[intro]: "cleaned op \<Longrightarrow> cleaned (Write op q x)"
+| cleaned_End[iff]: "cleaned End"
+
+inductive_cases cleaned_ReadE[elim!]: "cleaned (Read p f)"
+inductive_cases cleaned_WriteE[elim!]: "cleaned (Write op q x)"
+inductive_cases cleaned_EndE[elim!]: "cleaned End"
+
+inductive cleaned_cong for R where
+  cc_base: "R op \<Longrightarrow> cleaned_cong R op"
+| cc_cleaned: "cleaned op \<Longrightarrow> cleaned_cong R op"
+| cc_read: "p \<notin> inputs (f EOS) \<Longrightarrow> (\<And>x. cleaned_cong R (f x)) \<Longrightarrow> cleaned_cong R (Read p f)"
+| cc_write: "cleaned_cong R op \<Longrightarrow> cleaned_cong R (Write op q x)"
+
+lemma cleaned_coinduct_upto: "X op \<Longrightarrow>
+  (\<And>op. X op \<Longrightarrow> (\<exists>p f. op = Read p f \<and> p \<notin> inputs (f EOS) \<and> (\<forall>x. cleaned_cong X (f x))) \<or> (\<exists>op' q x. op = Write op' q x \<and> (cleaned_cong X op')) \<or> op = End) \<Longrightarrow>
+  cleaned op"
+  apply (rule cleaned.coinduct[where X="cleaned_cong X"])
+   apply (erule cleaned_cong.intros)
+  apply (erule thin_rl)
+  subgoal premises prems for op
+    using prems(2)
+    apply (induct op rule: cleaned_cong.induct)
+    subgoal for op
+      by (auto dest: prems(1))
+    subgoal for op
+      by (cases op) auto
+    subgoal for f p
+      by auto
+    subgoal for f p
+      by auto
+    done
+  done
+
+lemma ldropn_LConsD: "ldropn n xs = LCons x ys \<Longrightarrow> x \<in> lset xs"
+  by (metis in_lset_ldropnD lset_intros(1))
+
+lemma non_input_traces: "t \<in> lset lxs \<Longrightarrow> t = (Inp p, y) \<Longrightarrow> p \<notin> inputs op \<Longrightarrow> lxs \<in> traces m op \<Longrightarrow> False"
+  apply (induct t lxs arbitrary: m op rule: llist.set_induct)
+  subgoal for t lxs m op
+    apply (cases op; auto)
+    done
+  subgoal for t lxs x m op
+    apply (cases op; auto split: nat.splits)
+    done
+  done
+
+lemma cleaned_traced_gen:
+  "cleaned op \<Longrightarrow> traced m op (rev ps @@- lxs) \<Longrightarrow> alw (wow ((=) (Inp p, EOS)) imp nxt (alw (wow (\<lambda>t. fst t \<noteq> Inp p)))) ps lxs"
+  apply (coinduction arbitrary: m op ps lxs)
+  subgoal for m op ps lxs
+    apply (cases lxs)
+     apply simp_all
+    subgoal for x lxs'
+      apply (intro conjI impI disjI1; blast?)
+      apply (induct ps arbitrary: op m rule: rev_induct)
+       apply simp
+       apply (erule traced.cases; simp)
+       apply (erule cleaned.cases; simp)
+       apply (auto simp: alw_iff_ldropn wow_alt dest!: ldropn_LConsD dest: non_input_traces[unfolded traces_def] split: llist.splits) []
+      apply simp
+      apply (erule traced.cases; simp)
+         apply (erule cleaned.cases; auto simp add: alw_iff_ldropn wow_alt)+
+      done
+    done
+  done
+
+lemma cleaned_traced:
+  "cleaned op \<Longrightarrow> traced m op lxs \<Longrightarrow> alw (wow ((=) (Inp p, EOS)) imp nxt (alw (wow (\<lambda>t. fst t \<noteq> Inp p)))) [] lxs"
+  using cleaned_traced_gen[where ps = "[]"] by simp
+
+section\<open>Trace model full abstraction\<close>
+
+lemma traced_traced_wit: "traced m op (traced_wit op)"
+  apply (coinduction arbitrary: op m)
+  apply (subst (1 3 5 7) traced_wit.code)
+  apply (auto split: op.splits dest: lset_traced_wit simp: traced_wit.code[where op=End])
+  done
+
+lemma traces_nonempty: "traces m op \<noteq> {}"
+  by (auto simp: traces_def intro!: traced_traced_wit)
+
+lemma traces_op_eqI: "(\<Union>m. traces m op) = (\<Union>m. traces m op') \<Longrightarrow> op = op'"
+  apply (coinduction arbitrary: op op')
+  subgoal for op op'
+    apply (cases op; cases op')
+            apply (simp_all add: rel_fun_def set_eq_iff split: nat.splits)
+    subgoal for p f p' f'
+      apply (rule context_conjI)
+      subgoal
+        apply (drule spec[of _ "LCons (Inp p, EOS) (traced_wit (f EOS))"])
+        apply simp
+        apply (drule iffD1)
+         apply (rule exI[of _ "\<lambda>_. 0"])
+         apply simp
+         apply (rule disjI2)
+         apply (rule imageI)
+         apply (auto dest: lset_traced_wit simp: traces_def traced_traced_wit) []
+        apply (erule exE disjE conjE)+
+         apply (simp_all add: gr0_conv_Suc image_iff)
+        done
+      subgoal
+        apply safe
+        subgoal for x lxs m
+          apply (drule spec[of _ "LCons (Inp p, x) lxs"])
+          apply (drule iffD1)
+           apply (rule exI[of _ "m(p := Suc (m p))"])
+           apply (cases x; auto simp: image_iff dest: non_input_traces intro: exI[of _ "m p"]) []
+          apply (erule exE conjE disjE)+
+           apply (auto simp add: gr0_conv_Suc image_iff)
+          done
+        subgoal for x lxs m
+          apply (drule spec[of _ "LCons (Inp p', x) lxs"])
+          apply (drule iffD2)
+           apply (rule exI[of _ "m(p' := Suc (m p'))"])
+           apply (cases x; auto simp: image_iff dest: non_input_traces intro: exI[of _ "m p'"]) []
+          apply (erule exE conjE disjE)+
+           apply (auto simp add: gr0_conv_Suc image_iff)
+          done
+        done
+      done
+    subgoal
+      apply (auto simp: set_eq_iff image_iff)
+      apply (metis (no_types, lifting) IO.distinct(1) llist.inject mem_Collect_eq prod.inject traced_traced_wit traces_def)
+      done
+    subgoal
+      apply (auto dest!: spec[of _ LNil] simp: gr0_conv_Suc)
+      done
+    subgoal
+      apply (auto simp: set_eq_iff image_iff)
+      apply (metis (no_types, lifting) IO.distinct(1) llist.inject mem_Collect_eq prod.inject traced_traced_wit traces_def)
+      done
+    subgoal for op1 p1 x1 op2 p2 x2
+      apply auto
+      subgoal for lxs m
+        apply (drule spec[of _ "LCons (Out p1, Observed x1) lxs"])
+        apply auto
+        done
+      subgoal for lxs m
+        apply (drule spec[of _ "LCons (Out p2, Observed x2) lxs"])
+        apply auto
+        done
+      subgoal
+        apply (drule spec[of _ "LCons (Out p1, Observed x1) (traced_wit op1)"])
+        apply (auto simp: traced_traced_wit traces_def)
+        done
+      subgoal
+        apply (drule spec[of _ "LCons (Out p1, Observed x1) (traced_wit op1)"])
+        apply (auto simp: traced_traced_wit traces_def)
+        done
+      done
+    subgoal
+      apply (auto simp: set_eq_iff image_iff)
+      done
+    subgoal
+      apply (auto dest!: spec[of _ LNil] simp: gr0_conv_Suc)
+      done
+    subgoal
+      apply (auto simp: set_eq_iff image_iff)
+      done
+    done
+  done
+
+section\<open>Produce function\<close>
+
+inductive producing for p where
+  "producing p End lxs 0"
+| "producing p (Write _ p _) lxs 0"
+| "producing p (f (CHD p' lxs)) (CTL p' lxs) i \<Longrightarrow> producing p (Read p' f) lxs (Suc i)"
+| "p \<noteq> p' \<Longrightarrow> producing p op lxs i \<Longrightarrow> producing p (Write op p' x) lxs (Suc i)"
+
+inductive_cases producing_EndE[elim!]: "producing p End lxs n"
+inductive_cases producing_WriteE[elim!]: "producing p (Write op p' x) lxs n"
+inductive_cases producing_ReadE[elim!]: "producing p (Read p' f) lxs n"
+
+lemma producing_inject: "producing p op lxs i \<Longrightarrow> producing p op lxs j \<Longrightarrow> i = j"
+  by (induct op lxs i arbitrary: j rule: producing.induct) fastforce+
+
+lemma The_producing: "producing p op lxs i \<Longrightarrow> The (producing p op lxs) = i"
+  using producing_inject by fast
+
+corecursive produce where
+  "produce op lxs p = (let produce' = (\<lambda>op' lxs'. if \<exists>i. producing p op lxs i then produce op' lxs' p else LNil) in case op of
+    Read p' f \<Rightarrow> (produce' (f (CHD p' lxs)) (CTL p' lxs))
+  | Write op' p' x \<Rightarrow> (if p = p' then LCons x (produce op' lxs p) else produce' op' lxs)
+  | End \<Rightarrow> LNil)"
+  by (relation "measure (\<lambda>(op, lxs, p). THE i. producing p op lxs i)")
+    (auto 0 3 simp: The_producing del: producing_ReadE producing_WriteE elim: producing.cases)
+
+lemma produce_code[code]:
+  "produce op lxs p = (case op of
+    Read p' f \<Rightarrow> produce (f (CHD p' lxs)) (CTL p' lxs) p
+  | Write op' p' x \<Rightarrow> (if p = p' then LCons x (produce op' lxs p) else produce op' lxs p)
+  | End \<Rightarrow> LNil)"
+  apply (subst produce.code)
+  apply (simp split: op.splits if_splits)
+  apply safe
+  subgoal for p' f
+    by (subst produce.code) (auto 0 5 split: op.splits intro: producing.intros)
+  subgoal for op p x
+    by (subst produce.code) (auto 0 4 split: op.splits intro: producing.intros)
+  done
+
+simps_of_case produce_simps[simp]: produce_code
+
+(* lemma produced_produce: "produced m op lxs (produce op lxs)"
+  apply (coinduction arbitrary: m op lxs)
+  subgoal for m op lxs
+    by (cases op) (force simp: muted_def muted_produce[unfolded muted_def])+
+  done *)
+
+
+section\<open>History model\<close>
+
+definition "history op lxs lys =
+  (\<exists> ios m. traced m op ios \<and>
+  (\<forall> p. lprefix (lproject (\<lambda>p q. Inp p = q) ios p) (lxs p)) \<and> lys = lproject (\<lambda>p q. Out p = q) ios)"
+
+corec produce_trace where
+  "produce_trace op lxs = (case op of
+    Read p f \<Rightarrow> LCons (Inp p, CHD p lxs) (produce_trace (f (CHD p lxs)) (CTL p lxs))
+  | Write op' p x \<Rightarrow> LCons (Out p, Observed x) (produce_trace op' lxs)
+  | End \<Rightarrow> LNil)"
+
+simps_of_case produce_trace_simps[simp]: produce_trace.code
+
+lemma lset_produce_trace_not_LNil:
+  "r \<in> lset (produce_trace op lxs) \<Longrightarrow>
+   r = (Inp p, x) \<Longrightarrow>
+   x \<noteq> EOS \<Longrightarrow>
+   lxs p \<noteq> LNil"
+  apply (induct "produce_trace op lxs" arbitrary: op lxs rule: lset_induct[where x=r])
+  subgoal for xs op lxs
+    apply hypsubst_thin
+    apply (cases op)
+      apply (auto split: op.splits)
+    done
+  subgoal for x xs op lxs
+    apply hypsubst_thin
+    apply (cases op)
+      apply (auto split: op.splits)
+     apply fastforce
+    apply (metis fun_upd_other fun_upd_same ltl_simps(1))
+    done
+  done
+
+lemma lset_produce_trace_lhd:
+  "r \<in> lset (produce_trace op lxs) \<Longrightarrow>
+   r = (Inp p, Observed x) \<Longrightarrow>
+   lhd (lproject (\<lambda>p. (=) (Inp p)) (produce_trace op lxs) p) = lhd (lxs p)"
+  apply (induct "produce_trace op lxs" arbitrary: op lxs rule: lset_induct[where x=r])
+  subgoal for xs op lxs
+    apply hypsubst_thin
+    apply (cases op)
+      apply (auto split: op.splits)
+    apply (smt (verit, best) chd.elims eq_LConsD lproject_LCons(1) observation.disc(3) observation.discI)
+    done
+  subgoal for x xs op lxs
+    apply hypsubst_thin
+    apply (cases op)
+      apply (auto split: op.splits)
+    apply (smt (z3) IO.inject(1) chd.elims eq_LConsD fun_upd_other fun_upd_triv lproject_LCons(1) lproject_LCons(2) ltl_simps(1))
+    done
+  done
+
+
+lemma EOB_not_ind_produce_trace[simp]:
+  "(Inp p, EOB) \<notin> lset (produce_trace op lxs)"
+  unfolding not_def
+  apply (rule impI)
+  apply (induct "produce_trace op lxs" arbitrary: op lxs rule: lset_induct)
+  subgoal for xs op lxs
+    apply (cases op)
+      apply (auto simp add: split_beta split: observation.splits prod.splits)
+    apply (metis chd.elims observation.simps(3) observation.simps(7))
+    done
+  subgoal for x xs op lxs
+    apply (cases op)
+      apply (auto simp add: split_beta split: observation.splits prod.splits)
+    done
+  done
+
+inductive input_along where
+  "input_along p (Read p f) lxs"
+| "p \<noteq> p' \<Longrightarrow> input_along p (f (CHD p' lxs)) (CTL p' lxs) \<Longrightarrow> input_along p (Read p' f) lxs"
+| "input_along p op' lxs \<Longrightarrow> input_along p (Write op' p' x) lxs"
+
+lemma input_along_evidence:
+  "(Inp p, Observed x) \<in> lset (produce_trace op lxs) \<Longrightarrow>
+   input_along p op lxs"
+  apply (induct "produce_trace op lxs" arbitrary: op lxs rule: lset_induct)
+  subgoal for xs op lxs
+    apply (cases op)
+      apply (auto intro: input_along.intros)
+    done
+  subgoal for x' xs op lxs
+    apply (cases op)
+      apply (auto intro: input_along.intros)
+    done
+  done
+
+lemma
+  "history op lxs (produce op lxs)"
+  unfolding history_def
+  apply (rule exI[of _ "produce_trace op lxs"])
+  apply (rule exI[of _ "SOME m. traced m op (produce_trace op lxs)"])
+  apply (intro impI conjI allI)
+  subgoal sorry
+  subgoal for p
+    apply (coinduction arbitrary: op lxs rule: lprefix_coinduct)
+    subgoal for op lxs
+      apply (intro disjI1 impI conjI)
+      subgoal
+        by (auto simp add: lproject_empty_conv(1) lnull_def dest: lset_produce_trace_not_LNil intro: lproject_False elim!: chd.elims)
+      subgoal
+        by (auto simp add: lproject_empty_conv(1) lnull_def dest: lset_produce_trace_lhd intro: lproject_False elim!: chd.elims)
+      subgoal
+        apply (subgoal_tac "input_along p op lxs")
+        subgoal
+          apply (rotate_tac 2)
+          apply (induct p op lxs rule: input_along.induct)
+            apply simp_all
+          apply (smt (verit, best) chd.elims fun_upd_same lnull_def lproject_LCons(1) ltl_simps(2))
+          done
+        subgoal
+          using input_along_evidence lnull_def lproject_empty_conv(1) by fastforce
+        done
+      done
+    done
+  subgoal
+    oops
+
+
+    section\<open>Buffer infrastrcuture\<close>
+
+datatype 'd buf = BEmpty | BEnded | BCons 'd "'d buf"
+
+fun bhd where
+  "bhd BEmpty = EOB"
+| "bhd BEnded = EOS"
+| "bhd (BCons x xs) = Observed x"
+
+fun btl where
+  "btl BEmpty = BEmpty"
+| "btl BEnded = BEnded"
+| "btl (BCons x xs) = xs"
+
+fun bend where
+  "bend BEmpty = BEnded"
+| "bend BEnded = BEnded"
+| "bend (BCons xs xss) = BCons xs (bend xss)"
+
+fun benq where
+  "benq x BEmpty = BCons x BEmpty"
+| "benq x BEnded = BCons x BEnded"
+| "benq x (BCons y ys) = BCons y (benq x ys)"
+
+abbreviation BHD :: "'a \<Rightarrow> ('a \<Rightarrow> 'd buf) \<Rightarrow> 'd observation" where "BHD p buf \<equiv> bhd (buf p)"
+abbreviation (input) BUPD where "BUPD f p buf \<equiv> buf(p := f (buf p))"
+abbreviation BTL :: "'a \<Rightarrow> ('a \<Rightarrow> 'd buf) \<Rightarrow> ('a \<Rightarrow> 'd buf)" where "BTL \<equiv> BUPD btl"
+abbreviation BENQ :: "'a \<Rightarrow> 'd \<Rightarrow> ('a \<Rightarrow> 'd buf) \<Rightarrow> ('a \<Rightarrow> 'd buf)" where "BENQ p x buf \<equiv> BUPD (benq x) p buf"
+abbreviation BENQ_TL :: "'a \<Rightarrow> 'd \<Rightarrow> ('a \<Rightarrow> 'd buf) \<Rightarrow> ('a \<Rightarrow> 'd buf)" where "BENQ_TL p x buf \<equiv> BUPD (btl o benq x) p buf"
+
+fun bapp where
+  "bapp BEmpty lxs = lxs"
+| "bapp BEnded lxs = LNil"
+| "bapp (BCons x xs) lxs = LCons x (bapp xs lxs)"
+
+definition "extend A buf R lxs lys =
+  (\<exists>lzs. R lxs (case_sum (lys o Inl) lzs) \<and> (\<forall>p. lys (Inr p) = (if p \<in> A then bapp (buf p) (lzs p) else lzs p)))"
+
+lemma extend_empty: "extend {} buf R = R"
+  using arg_cong2[of x x "case_sum (f o Inl) (f o Inr)" f R for x f, unfolded o_def, OF refl surjective_sum]
+  by (auto simp: extend_def o_def fun_eq_iff[of "extend _ _ _"] fun_eq_iff[of "extend _ _ _ _"]
+      simp flip: fun_eq_iff split: sum.splits)
 
 section\<open>Well-typed\<close>
 
@@ -542,7 +672,7 @@ coinductive welltyped where
 inductive_cases welltyped_ReadE[elim!]: "welltyped A B (Read p f)"
 inductive_cases welltyped_WriteE[elim!]: "welltyped A B (Write op q x)"
 inductive_cases welltyped_EndE[elim!]: "welltyped A B End"
-(*
+  (*
 (*characteristic property of welltyped*)
 lemma "x \<in> lset (lproject (=) lxs (Out q)) \<Longrightarrow> traced m op lxs \<Longrightarrow> welltyped A B op \<Longrightarrow> \<forall>p. lset (lproject (=) lxs (Inp p)) \<subseteq> A p \<Longrightarrow> x \<in> B q"
   apply (induct x "lproject (=) lxs (Out q)" arbitrary: m op lxs rule: llist.set_induct)
